Java/src/Java/Tactics/Tactics.v
@@ -119,85 +119,85 @@ End Tactics.
 
 Definition my_exprD' := @exprD' typ RType_typ (expr typ func).
 
-
-Print Transparent Dependencies my_exprD'.
-
 Ltac cbv_denote :=
-          cbv [
-          goalD_aux
-          
-		  (* ExprD' *)
-          exprD' symAs  typeof_sym typeof_expr type_cast type_cast_typ
-          exprD'_simul func_simul
-          Expr.Expr_expr
-          ExprDsimul.ExprDenote.exprD'
-          (* RSym *)
-          
-          SymSum.RSym_sum Rcast Relim Rsym eq_sym symD(* RSym_env*)
-          Rcast_val eq_rect_r eq_rect Datatypes.id
-          RSym_Empty RSymOneOf typeof_sym_OneOf symD_OneOf sym_eqb_OneOf
-          (* Monad *)
-          
-          Monad.bind Monad.ret
-          
-          OptionMonad.Monad_option
-          
-          (* HList *)
-          
-          HList.hlist_hd HList.hlist_tl
-          
-          (* TypesI *)
-          
-          TypesI.typD 
-          typ2_match typ2 typ2_cast
-          typ0_match typ0 typ0_cast
-          castR castD
-          (* ExprI *)
-          
-          MirrorCore.VariablesI.Var ExprVariables.ExprVar_expr
-          MirrorCore.VariablesI.UVar
-          MirrorCore.Lambda.ExprVariables.ExprUVar_expr
-          ExprI.exprT_Inj ExprI.exprT_UseV ExprI.exprT_UseU
-          exprT_App ExprI.exprT OpenT
-          nth_error_get_hlist_nth
-          
-          exprT_GetVAs exprT_GetUAs
-          
-          (* ILogicView*)
-          
-          ILogicView.mkEntails ILogicView.mkTrue ILogicView.mkFalse 
-          ILogicView.mkAnd ILogicView.mkOr ILogicView.mkImpl
-          ILogicView.mkExists ILogicView.mkForall
-          
-          ILogicView.fEntails ILogicView.fTrue ILogicView.fFalse ILogicView.fAnd 
-          ILogicView.fOr ILogicView.fImpl ILogicView.fExists ILogicView.fForall
-          ILogicView.RSym_ilfunc 
-          
-          ILogicView.funcD
-	  ILogicView.trueR
-	  ILogicView.falseR
-	  ILogicView.andR
-	  ILogicView.orR
-	  ILogicView.existsR
-	  ILogicView.forallR
-          
-          (* BILogicFunc *)
-          
-          BILogicView.mkEmp BILogicView.mkStar BILogicView.mkWand
-          
-          BILogicView.fEmp BILogicView.fStar BILogicView.fWand
-          
-          BILogicView.RSym_bilfunc
-          
-          BILogicView.funcD
-	  BILogicView.empR
-	  BILogicView.starR
-	  BILogicView.wandR
-          
-          BILogicView.typeof_bilfunc
-          
-          (* LaterFunc *)
-          (*
+  cbv [
+      goalD_aux
+        
+	(* ExprD' *)
+        exprD' symAs  typeof_sym typeof_expr type_cast type_cast_typ
+        exprD'_simul func_simul
+        Expr.Expr_expr
+        ExprDsimul.ExprDenote.exprD'
+        (* RSym *)
+        
+        SymSum.RSym_sum Rcast Relim Rsym eq_sym symD(* RSym_env*)
+        Rcast_val eq_rect_r eq_rect Datatypes.id
+        RSym_Empty RSymOneOf typeof_sym_OneOf symD_OneOf sym_eqb_OneOf
+        (* Monad *)
+        
+        Monad.bind Monad.ret
+        
+        OptionMonad.Monad_option
+        
+        (* HList *)
+        
+        HList.hlist_hd HList.hlist_tl
+        
+        (* TypesI *)
+        TypesI.Typ1_App
+        TypesI.Typ2_App
+        TypesI.typD 
+        typ2_match typ2 typ2_cast
+        typ1_match typ1 typ1_cast
+        typ0_match typ0 typ0_cast
+        castR castD
+        (* ExprI *)
+        
+        MirrorCore.VariablesI.Var ExprVariables.ExprVar_expr
+        MirrorCore.VariablesI.UVar
+        MirrorCore.Lambda.ExprVariables.ExprUVar_expr
+        ExprI.exprT_Inj ExprI.exprT_UseV ExprI.exprT_UseU
+        exprT_App ExprI.exprT OpenT
+        HList.nth_error_get_hlist_nth 
+        
+        exprT_GetVAs exprT_GetUAs
+        
+        (* ILogicView*)
+        
+        ILogicView.mkEntails ILogicView.mkTrue ILogicView.mkFalse 
+        ILogicView.mkAnd ILogicView.mkOr ILogicView.mkImpl
+        ILogicView.mkExists ILogicView.mkForall
+        
+        ILogicView.fEntails ILogicView.fTrue ILogicView.fFalse ILogicView.fAnd 
+        ILogicView.fOr ILogicView.fImpl ILogicView.fExists ILogicView.fForall
+        ILogicView.RSym_ilfunc 
+        
+        ILogicView.funcD
+        ILogicView.entailsR
+	ILogicView.trueR
+	ILogicView.falseR
+	ILogicView.andR
+	ILogicView.orR
+	ILogicView.existsR
+	ILogicView.forallR
+        
+        (* BILogicFunc *)
+        
+        BILogicView.mkEmp BILogicView.mkStar BILogicView.mkWand
+        
+        BILogicView.fEmp BILogicView.fStar BILogicView.fWand
+        
+        BILogicView.RSym_bilfunc
+        
+        BILogicView.funcD
+	BILogicView.empR
+	BILogicView.starR
+	BILogicView.wandR
+        
+        BILogicView.typeof_bilfunc
+        
+        (* LaterFunc *)
+        (*
           LaterFunc.mkLater
           
           LaterFunc.fLater
@@ -209,199 +209,207 @@ Ltac cbv_denote :=
           
           LaterFunc.typeof_later_func
           
-          (* EmbedFunc *)
-          *)
-          EmbedView.mkEmbed
+         (* EmbedFunc *)
+         *)
+        EmbedView.mkEmbed
+        
+        EmbedView.fEmbed
+        
+        EmbedView.RSym_embed_func 
+        
+        EmbedView.funcD 
+        
+	EmbedView.embedD
+        
+        EmbedView.typeof_embed_func
+        
+        (* EqView *)
+        
+        EqView.mkCons EqView.fEq EqView.RSym_EqFunc EqView.eq_func_symD EqView.eqR EqView.typeof_eq_func
+        EqView.eq_func_eq EqView.typeof_eq_func
+        
+        (* StringView *)
+        
+        StringView.fString
+        StringView.mkString
+        
+        StringView.RSym_StringFunc StringView.string_func_symD
+        
+        StringView.stringR
+        
+        StringView.typeofStringFunc
+        
+        (* NatView *)
+        
+        NatView.fNat
+        NatView.mkNat
+        
+        NatView.RSym_NatFunc NatView.nat_func_symD
+        
+        NatView.natR
+        
+        NatView.typeofNatFunc
+        
+        (* BoolView *)
+        
+        BoolView.fBool
+        BoolView.mkBool
+        
+        BoolView.RSym_BoolFunc BoolView.bool_func_symD
+        
+        BoolView.boolR
+        
+        BoolView.typeofBoolFunc
+        (* BoolView *)
+        
+        BoolView.fBool
+        BoolView.mkBool
+        
+        BoolView.RSym_BoolFunc BoolView.bool_func_symD
+        
+        BoolView.boolR
+        
+        BoolView.typeofBoolFunc
+        
+        (* ProdView *)
+        
+        ProdView.fPair
+        ProdView.mkPair
+        
+        ProdView.RSym_ProdFunc ProdView.prod_func_symD
+        
+        ProdView.pairR
+        
+        ProdView.typeof_prod_func
+        
+        (* ListView *)
+        
+        ListView.fNil ListView.fCons
+        ListView.mkNil ListView.mkCons
+        
+        ListView.RSym_ListFunc ListView.list_func_symD
+        
+        ListView.nilR ListView.consR
+        
+        ListView.typeof_list_func
+        
+        (* ListOpView *)
+        
+        ListOpView.fLength ListOpView.fNoDup ListOpView.fIn
+        ListOpView.fMap ListOpView.fFold ListOpView.fCombine
+        
+        ListOpView.mkLength ListOpView.mkNoDup ListOpView.mkIn
+        ListOpView.mkMap ListOpView.mkFold ListOpView.mkCombine
+        
+        ListOpView.RSym_ListOpFunc ListOpView.listOp_func_symD
+        
+        ListOpView.lengthR ListOpView.NoDupR ListOpView.InR
+        ListOpView.mapR ListOpView.foldR ListOpView.combineR
+        
+        
+        ListOpView.typeof_listOp_func
           
-          EmbedView.fEmbed
+        (* ApView *)
+        
+        ApplicativeView.fPure ApplicativeView.fAp
+        ApplicativeView.mkPure ApplicativeView.mkAp
           
-          EmbedView.RSym_embed_func 
-          
-          EmbedView.funcD 
-          
-	  EmbedView.embedD
-
-          EmbedView.typeof_embed_func
-          
-          (* StringView *)
-          
-          StringView.fString
-          StringView.mkString
-
-          StringView.RSym_StringFunc StringView.string_func_symD
-
-          StringView.stringR
-
-          StringView.typeofStringFunc
-          
-          (* NatView *)
-          
-          NatView.fNat
-          NatView.mkNat
-
-          NatView.RSym_NatFunc NatView.nat_func_symD
-
-          NatView.natR
-
-          NatView.typeofNatFunc
-          
-          (* BoolView *)
-          
-          BoolView.fBool
-          BoolView.mkBool
-
-          BoolView.RSym_BoolFunc BoolView.bool_func_symD
-
-          BoolView.boolR
-
-          BoolView.typeofBoolFunc
-          (* BoolView *)
-          
-          BoolView.fBool
-          BoolView.mkBool
-
-          BoolView.RSym_BoolFunc BoolView.bool_func_symD
-
-          BoolView.boolR
-
-          BoolView.typeofBoolFunc
-          
-          (* ProdView *)
-          
-          ProdView.fPair
-          ProdView.mkPair
-
-          ProdView.RSym_ProdFunc ProdView.prod_func_symD
-
-          ProdView.pairR
-
-          ProdView.typeof_prod_func
-          
-          (* ListView *)
-          
-          ListView.fNil ListView.fCons
-          ListView.mkNil ListView.mkCons
-
-          ListView.RSym_ListFunc ListView.list_func_symD
-
-          ListView.nilR ListView.consR
-
-          ListView.typeof_list_func
-          
-          (* ListOpView *)
-          
-          ListOpView.fLength ListOpView.fNoDup ListOpView.fIn
-          ListOpView.fMap ListOpView.fFold ListOpView.fCombine
-
-          ListOpView.mkLength ListOpView.mkNoDup ListOpView.mkIn
-          ListOpView.mkMap ListOpView.mkFold ListOpView.mkCombine
-
-          ListOpView.RSym_ListOpFunc ListOpView.listOp_func_symD
-
-          ListOpView.lengthR ListOpView.NoDupR ListOpView.InR
-          ListOpView.mapR ListOpView.foldR ListOpView.combineR
-
-
-          ListOpView.typeof_listOp_func
-          
-          (* ApView *)
-          
-          ApplicativeView.fPure ApplicativeView.fAp
-          ApplicativeView.mkPure ApplicativeView.mkAp
-
-          ApplicativeView.RSym_ApFunc ApplicativeView.ap_func_symD
-
-          ApplicativeView.pureR ApplicativeView.apR
-
-          ApplicativeView.typeof_ap_func
-          
-	  (* OpenFunc *)
+        ApplicativeView.RSym_ApFunc ApplicativeView.ap_func_symD
+        
+        ApplicativeView.pureR ApplicativeView.apR
+        
+        ApplicativeView.typeof_ap_func
+        
+	(* OpenFunc *)
+	
+	SubstView.mkNull SubstView.mkStackGet
+	SubstView.mkStackSet SubstView.mkApplySubst SubstView.mkSingleSubst SubstView.mkSubst
+	SubstView.mkTruncSubst
+	
+	SubstView.fNull SubstView.fStackGet
+	SubstView.fApplySubst SubstView.fSingleSubst SubstView.fSubst SubstView.fTruncSubst
 	  
-	  SubstView.mkNull SubstView.mkStackGet
-	  SubstView.mkStackSet SubstView.mkApplySubst SubstView.mkSingleSubst SubstView.mkSubst
-	  SubstView.mkTruncSubst
-	  
-	  SubstView.fNull SubstView.fStackGet
-	  SubstView.fApplySubst SubstView.fSingleSubst SubstView.fSubst SubstView.fTruncSubst
-	  
-	  SubstView.open_func_symD
-	  
-	  SubstView.typeof_subst_func SubstView.RSym_SubstFunc
-          
-	  SubstView.stack_getR
-	  SubstView.stack_setR
-	  SubstView.applySubstR
-	  SubstView.singleSubstR
-		  
-          
-          (* JavaType *)
+	SubstView.open_func_symD
+	
+	SubstView.typeof_subst_func SubstView.RSym_SubstFunc
+        
+	SubstView.stack_getR
+	SubstView.stack_setR
+	SubstView.applySubstR
+	SubstView.singleSubstR
+	
+        
+        (* JavaType *)
          
-          Typ2_Fun Typ0_Prop RType_typ typD
-          should_not_be_necessary should_also_not_be_necessary
-         
-          JavaType.bilops JavaType.ilops
-          JavaType.eops (*JavaType.lops*)
+        Typ2_Fun Typ0_Prop RType_typ typD Typ0_string Typ0_bool
+        Typ0_val Typ0_nat Typ0_term Typ1_list Typ2_prod
+        should_not_be_necessary should_also_not_be_necessary
+        
+        JavaType.bilops JavaType.ilops
+        JavaType.eops (*JavaType.lops*)
+        
+        (*   JavaType.typD *)
+	(* JavaFunc *)
+        
+        
+        JavaFunc.RSym_ilfunc JavaFunc.RSym_bilfunc JavaFunc.RSym_embed_func
+        ilops (*is_pure*) func func_map RSym_JavaFunc typeof_java_func java_func_eq
+        java_func_symD RelDec_java_func typeof_ilfunc
+        list_to_pmap list_to_pmap_aux
+        JavaFunc.Expr_expr
+        mkPointstoVar
+        JavaFunc.RSym_sub_func
+        JavaFunc.RSym_func JavaFunc.java_env
+        JavaFunc.fVal JavaFunc.fFields
+        JavaFunc.fProg JavaFunc.fCmd JavaFunc.fDExpr JavaFunc.fFields
+        JavaFunc.fMethodSpec JavaFunc.fProgEq JavaFunc.fTriple JavaFunc.fTypeOf
+        JavaFunc.fFieldLookup JavaFunc.fPointsto JavaFunc.fNull
+        JavaFunc.fPlus JavaFunc.fMinus JavaFunc.fTimes JavaFunc.fAnd
+        JavaFunc.fOr JavaFunc.fNot JavaFunc.fLt JavaFunc.fValEq
+        JavaFunc.mkTriple JavaFunc.mkFieldLookup JavaFunc.mkTypeOf
+        JavaFunc.mkProgEq JavaFunc.mkExprList JavaFunc.evalDExpr
+        
+        (* OTHER *)
+        
+        goalD Ctx.propD propD exprD'_typ0 exprD split_env
+        
+        amap_substD
+        substD
+        SUBST.raw_substD
+        UVarMap.MAP.fold
+        FMapPositive.PositiveMap.fold
+        FMapPositive.PositiveMap.xfoldi
+        FMapPositive.append
+        UVarMap.MAP.from_key
+        pred
+        plus
+        Pos.to_nat
+        Pos.succ
+        Pos.iter_op
+        List.app
+        HList.hlist_app
+        Quant._foralls
+        Quant._exists
+        goalD_Prop
           
-       (*   JavaType.typD *)
-		 (* JavaFunc *)
-          
-
-          JavaFunc.RSym_ilfunc JavaFunc.RSym_bilfunc JavaFunc.RSym_embed_func
-          ilops (*is_pure*) func func_map RSym_JavaFunc typeof_java_func java_func_eq
-          java_func_symD RelDec_java_func typeof_ilfunc
-          list_to_pmap list_to_pmap_aux
-          JavaFunc.Expr_expr
-          mkPointstoVar
-          JavaFunc.RSym_sub_func
-          JavaFunc.RSym_func JavaFunc.java_env
-          JavaFunc.fVal JavaFunc.fFields
-          JavaFunc.fProg JavaFunc.fCmd JavaFunc.fDExpr JavaFunc.fFields
-          JavaFunc.fMethodSpec JavaFunc.fProgEq JavaFunc.fTriple JavaFunc.fTypeOf
-          JavaFunc.fFieldLookup JavaFunc.fPointsto JavaFunc.fNull
-          JavaFunc.fPlus JavaFunc.fMinus JavaFunc.fTimes JavaFunc.fAnd
-          JavaFunc.fOr JavaFunc.fNot JavaFunc.fLt JavaFunc.fValEq
-          JavaFunc.mkTriple JavaFunc.mkFieldLookup JavaFunc.mkTypeOf
-          JavaFunc.mkProgEq JavaFunc.mkExprList JavaFunc.evalDExpr
-          
-(* OTHER *)
-  
-          goalD Ctx.propD propD exprD'_typ0 exprD split_env
-          
-          amap_substD
-          substD
-          SUBST.raw_substD
-          UVarMap.MAP.fold
-          FMapPositive.PositiveMap.fold
-          FMapPositive.PositiveMap.xfoldi
-          FMapPositive.append
-          UVarMap.MAP.from_key
-          pred
-          plus
-          Pos.to_nat
-          Pos.iter_op
-          app
-          HList.hlist_app
-          Quant._foralls
-          Quant._exists
-          goalD_Prop
-
-          FuncView.f_insert
-          SumN.pmap_lookup'
-
-          (* FMapPositive *)
-          FMapPositive.pmap_here
-          FMapPositive.pmap_left
-          FMapPositive.pmap_right
-          FMapPositive.pmap_lookup
-          FMapPositive.pmap_insert
-          FMapPositive.branch
-          FMapPositive.pmap_remove
-          FMapPositive.pmap_empty
-          FMapPositive.pmap_union
-
-          Pos.add
-          SymOneOf.internal_eq_rew_dep
-          ].
+        FuncView.f_insert
+        SumN.pmap_lookup'
+        
+        (* FMapPositive *)
+        FMapPositive.pmap_here
+        FMapPositive.pmap_left
+        FMapPositive.pmap_right
+        FMapPositive.pmap_lookup
+        FMapPositive.pmap_insert
+        FMapPositive.branch
+        FMapPositive.pmap_remove
+        FMapPositive.pmap_empty
+        FMapPositive.pmap_union
+        
+        Pos.add
+        SymOneOf.internal_eq_rew_dep
+        
+    ].
 
 Let elem_ctor : forall x : typ, typD x -> @SymEnv.function _ _ :=
   @SymEnv.F _ _.
